src/paths-new/Substitution.v
@@ -27,7 +27,7 @@ Definition subst_avar (z: var) (u: path) (a: avar) : path :=
 
 (* p    [u / z] where p = x.bs:
    x.bs [u / z] == x [u / z] . bs *)
-Fixpoint subst_path (z: var) (u: path) (p: path) : path :=
+Definition subst_path (z: var) (u: path) (p: path) : path :=
   match p with
   | p_sel x bs => sel_fields (subst_avar z u x) bs
   end.
@@ -91,11 +91,17 @@ Proof.
   intros. destruct* a. simpl. autounfold. case_var*. simpls. notin_false.
 Qed.
 
-Lemma subst_fresh_path : forall x y p,
+Lemma subst_fresh_path : forall x q p,
     x \notin fv_path p ->
-    subst_path x y p = p.
+    subst_path x q p = p.
 Proof.
-  intros. destruct p. simpls. unfold subst_path. destruct a. Admitted.
+  intros. destruct p as [[n | z] bs]; simpls.
+  - Case "p = (avar_b n).bs".
+    rewrite* app_nil_r.
+  - Case "p = (avar_f z).bs".
+    unfold subst_var. apply notin_singleton in H. case_if.
+    simpl. rewrite* app_nil_r.
+Qed.
 
 (** - in types, declarations, paths *)
 Lemma subst_fresh_typ_dec: forall x y,
@@ -187,10 +193,10 @@ Proof.
     rewrite ((proj1 (subst_fresh_typ_dec _ _)) _ N1).
     reflexivity.
 Qed.
-
+(*
 (** Definition of substitution on named variables: #<br>#
     [z[y/x] := if z == x then y else z], where [z] is a named variable. *)
-Definition subst_fvar(x y z: var): var := If z = x then y else z.
+Definition subst_fvar(x y z: var): var := If z = x then y else z.*)
 
 (** The following lemmas state that substitution commutes with opening:
     for a symbol [Z], #<br>#
@@ -198,41 +204,72 @@ Definition subst_fvar(x y z: var): var := If z = x then y else z.
 
 (** Substitution commutes with opening
     - variables *)
-Lemma subst_open_commut: forall x y u a n,
-    subst_avar x y (open_rec_avar n u a)
-    = open_rec_avar n (subst_fvar x y u) (subst_avar x y a).
+Lemma subst_open_commut: forall x p u y n,
+    lc_path p ->
+    subst_avar x p (open_rec_avar n u y)
+    = open_rec_path_p n (subst_var x p u) (subst_avar x p y).
 Proof.
-  intros. unfold subst_fvar, subst_avar, open_avar, open_rec_avar. destruct a; autounfold.
-  + repeat case_if; auto.
-  + case_var*.
+  introv Hl. unfold subst_var, subst_avar, open_rec_avar, subst_var.
+  destruct y as [n' | y]; autounfold; destruct p as [z bs]; destruct z as [m | z'];
+    repeat case_if; simpl; try case_if*; eauto; inversions  Hl; inversions H0.
+Qed.
+
+Lemma sel_fields_open : forall n p q bs,
+  sel_fields (open_rec_path_p n p q) bs = open_rec_path_p n p (sel_fields q bs).
+Proof.
+  intros. destruct q. simpl. destruct p. destruct a. case_if; simpl; auto. rewrite* app_assoc.
+  simpl. auto.
 Qed.
 
 (** - paths *)
-Lemma subst_open_commut_path: forall p n x y u,
-     subst_path x y (open_rec_path n u p)
-     = open_rec_path n (subst_fvar x y u) (subst_path x y p).
+Lemma subst_open_commut_path: forall p n x q u,
+    lc_path p ->
+    subst_path x p (open_rec_path n u q)
+    = open_rec_path_p n (subst_var x p u) (subst_path x p q).
 Proof.
-  Admitted.
-
-(** - types and declarations *)
-Lemma subst_open_commut_typ_dec: forall x y u,
-  (forall t : typ, forall n: nat,
-     subst_typ x y (open_rec_typ n u t)
-     = open_rec_typ n (subst_fvar x y u) (subst_typ x y t)) /\
-  (forall D : dec, forall n: nat,
-     subst_dec x y (open_rec_dec n u D)
-     = open_rec_dec n (subst_fvar x y u) (subst_dec x y D)).
-Proof.
-  intros. apply typ_mutind; intros; simpl; f_equal*. apply subst_open_commut_path.
+  introv Hl. destruct q as [z bs]. simpl. rewrite* subst_open_commut. rewrite* sel_fields_open.
 Qed.
 
-Lemma subst_open_commut_path_p: forall p n x y u,
-    subst_path x y (open_rec_path_p n u p)
-    = open_rec_path_p n (subst_path x y u) (subst_path x y p).
+(** - types and declarations *)
+Lemma subst_open_commut_typ_dec: forall x p u,
+  lc_path p ->
+  (forall t : typ, forall n: nat,
+     subst_typ x p (open_rec_typ n u t)
+     = open_rec_typ_p n (subst_var x p u) (subst_typ x p t)) /\
+  (forall D : dec, forall n: nat,
+     subst_dec x p (open_rec_dec n u D)
+     = open_rec_dec_p n (subst_var x p u) (subst_dec x p D)).
 Proof.
-  intros. Admitted.
+  intros. apply typ_mutind; intros; simpl; f_equal*. apply* subst_open_commut_path.
+Qed.
+
+Lemma subst_open_commut_p: forall x p u y n,
+    lc_path p ->
+    subst_path x p (open_rec_avar_p n u y)
+    = open_rec_path_p n (subst_path x p u) (subst_avar x p y).
+Proof.
+  introv Hl. unfold subst_path, subst_avar, subst_var.
+  destruct y as [n' | y]; simpl; repeat case_if; destruct u; destruct a; simpl;
+    try (rewrite* app_nil_r); repeat case_if; unfold sel_fields; destruct* p;
+      inversions Hl; inversions H0; rewrite* app_nil_l.
+Qed.
+
+Lemma subst_open_commut_path_p: forall p n x q u,
+    lc_path q ->
+    subst_path x q (open_rec_path_p n u p)
+    = open_rec_path_p n (subst_path x q u) (subst_path x q p).
+Proof.
+  introv Hl. destruct p as [z bs]. simpl.
+  unfold subst_path. destruct u. rewrite <- sel_fields_open.
+  unfold open_rec_path_p, subst_avar.
+  destruct z; simpl; destruct a; repeat case_if*;
+    unfold subst_var; repeat case_if;
+      destruct q; simpl; try (rewrite app_assoc || rewrite app_nil_r);
+        try solve [inversion Hl; inversion* H0].
+Qed.
 
 Lemma subst_open_commut_typ_dec_p: forall x y u,
+  lc_path y ->
   (forall t : typ, forall n: nat,
      subst_typ x y (open_rec_typ_p n u t)
      = open_rec_typ_p n (subst_path x y u) (subst_typ x y t)) /\
@@ -241,42 +278,46 @@ Lemma subst_open_commut_typ_dec_p: forall x y u,
      = open_rec_dec_p n (subst_path x y u) (subst_dec x y D)).
 Proof.
   intros. apply typ_mutind; intros; simpl; f_equal*.
-  apply subst_open_commut_path_p.
+  apply* subst_open_commut_path_p.
 Qed.
 
 (** - types only *)
 Lemma subst_open_commut_typ: forall x y u T,
-  subst_typ x y (open_typ u T) = open_typ (subst_fvar x y u) (subst_typ x y T).
+  lc_path y ->
+  subst_typ x y (open_typ u T) = open_typ_p (subst_var x y u) (subst_typ x y T).
 Proof.
-  intros. apply subst_open_commut_typ_dec.
+  intros. apply* subst_open_commut_typ_dec.
 Qed.
 
 Lemma subst_open_commut_typ_p: forall x y u T,
-  subst_typ x y (open_typ_p u T) = open_typ_p (subst_path x y u) (subst_typ x y T).
+    lc_path y ->
+    subst_typ x y (open_typ_p u T) = open_typ_p (subst_path x y u) (subst_typ x y T).
 Proof.
   intros. apply* subst_open_commut_typ_dec_p.
 Qed.
 
 (** - terms, values, definitions, and list of definitions *)
 Lemma subst_open_commut_trm_val_def_defs: forall x y u,
+    lc_path y ->
   (forall t : trm, forall n: nat,
      subst_trm x y (open_rec_trm n u t)
-     = open_rec_trm n (subst_fvar x y u) (subst_trm x y t)) /\
+     = open_rec_trm_p n (subst_var x y u) (subst_trm x y t)) /\
   (forall v : val, forall n: nat,
      subst_val x y (open_rec_val n u v)
-     = open_rec_val n (subst_fvar x y u) (subst_val x y v)) /\
+     = open_rec_val_p n (subst_var x y u) (subst_val x y v)) /\
   (forall d : def , forall n: nat,
      subst_def x y (open_rec_def n u d)
-     = open_rec_def n (subst_fvar x y u) (subst_def x y d)) /\
+     = open_rec_def_p n (subst_var x y u) (subst_def x y d)) /\
   (forall ds: defs, forall n: nat,
      subst_defs x y (open_rec_defs n u ds)
-     = open_rec_defs n (subst_fvar x y u) (subst_defs x y ds)).
+     = open_rec_defs_p n (subst_var x y u) (subst_defs x y ds)).
 Proof.
   intros. apply trm_mutind; intros; simpl; f_equal*;
-  apply subst_open_commut_path || apply subst_open_commut_typ_dec.
+  apply* subst_open_commut_path || apply* subst_open_commut_typ_dec.
 Qed.
 
 Lemma subst_open_commut_trm_val_def_defs_p: forall x y u,
+    lc_path y ->
   (forall t : trm, forall n: nat,
      subst_trm x y (open_rec_trm_p n u t)
      = open_rec_trm_p n (subst_path x y u) (subst_trm x y t)) /\
@@ -291,18 +332,20 @@ Lemma subst_open_commut_trm_val_def_defs_p: forall x y u,
      = open_rec_defs_p n (subst_path x y u) (subst_defs x y ds)).
 Proof.
   intros. apply trm_mutind; intros; simpl; f_equal*;
-  apply subst_open_commut_typ_dec_p || apply subst_open_commut_path_p.
+  apply* subst_open_commut_typ_dec_p || apply* subst_open_commut_path_p.
 Qed.
 
 (** - terms only *)
 Lemma subst_open_commut_trm: forall x y u t,
+    lc_path y ->
     subst_trm x y (open_trm u t)
-    = open_trm (subst_fvar x y u) (subst_trm x y t).
+    = open_trm_p (subst_var x y u) (subst_trm x y t).
 Proof.
   intros. apply* subst_open_commut_trm_val_def_defs.
 Qed.
 
 Lemma subst_open_commut_trm_p: forall x y u t,
+    lc_path y ->
     subst_trm x y (open_trm_p u t)
     = open_trm_p (subst_path x y u) (subst_trm x y t).
 Proof.
@@ -311,13 +354,15 @@ Qed.
 
 (** - definitions only *)
 Lemma subst_open_commut_defs: forall x y u ds,
+    lc_path y ->
     subst_defs x y (open_defs u ds)
-    = open_defs (subst_fvar x y u) (subst_defs x y ds).
+    = open_defs_p (subst_var x y u) (subst_defs x y ds).
 Proof.
   intros. apply* subst_open_commut_trm_val_def_defs.
 Qed.
 
 Lemma subst_open_commut_defs_p: forall x y u ds,
+    lc_path y ->
     subst_defs x y (open_defs_p u ds)
     = open_defs_p (subst_path x y u) (subst_defs x y ds).
 Proof.
@@ -331,45 +376,45 @@ Qed.
 
 (** Substitution after opening
     - terms *)
-Lemma subst_intro_trm: forall x u t, x \notin (fv_trm t) ->
-  open_trm u t = subst_trm x u (open_trm x t).
+Lemma subst_intro_trm: forall x u t, x \notin (fv_trm t) -> lc_path u ->
+  open_trm_p u t = subst_trm x u (open_trm x t).
 Proof.
-  introv Fr. unfold open_trm. rewrite subst_open_commut_trm.
+  introv Fr Hl. unfold open_trm. rewrite* subst_open_commut_trm.
   destruct (@subst_fresh_trm_val_def_defs x u) as [Q _]. rewrite~ (Q t).
-  unfold subst_fvar. case_var~.
+  unfold subst_var. case_var~.
 Qed.
 
 (** - definitions *)
-Lemma subst_intro_defs: forall x u ds, x \notin (fv_defs ds) ->
-  open_defs u ds = subst_defs x u (open_defs x ds).
+Lemma subst_intro_defs: forall x u ds, x \notin (fv_defs ds) -> lc_path u ->
+  open_defs_p u ds = subst_defs x u (open_defs x ds).
 Proof.
-  introv Fr. unfold open_trm. rewrite subst_open_commut_defs.
+  introv Fr Hl. unfold open_trm. rewrite* subst_open_commut_defs.
   destruct (@subst_fresh_trm_val_def_defs x u) as [_ [_ [_ Q]]]. rewrite~ (Q ds).
-  unfold subst_fvar. case_var~.
+  unfold subst_var. case_var~.
 Qed.
 
 (** - types *)
-Lemma subst_intro_typ: forall x u T, x \notin (fv_typ T) ->
-  open_typ u T = subst_typ x u (open_typ x T).
+Lemma subst_intro_typ: forall x u T, x \notin (fv_typ T) -> lc_path u ->
+  open_typ_p u T = subst_typ x u (open_typ x T).
 Proof.
-  introv Fr. unfold open_typ. rewrite* subst_open_commut_typ.
+  introv Fr Hl. unfold open_typ. rewrite* subst_open_commut_typ.
   destruct (@subst_fresh_typ_dec x u) as [Q _]. rewrite* (Q T).
-  unfold subst_fvar. case_var*.
+  unfold subst_var. case_var*.
 Qed.
 
 Ltac subst_open_fresh :=
   repeat match goal with
     | [ |- context [ open_typ ?z (subst_typ ?x ?y ?T) ] ] =>
-        replace (open_typ z (subst_typ x y T)) with (open_typ (subst_fvar x y z) (subst_typ x y T))
-          by (unfold subst_fvar; rewrite~ If_r);
+        replace (open_typ z (subst_typ x y T)) with (open_typ (subst_var x y z) (subst_typ x y T))
+          by (unfold subst_var; rewrite~ If_r);
         rewrite_all <- subst_open_commut_typ
     | [ |- context [ open_defs ?z (subst_defs ?x ?y ?ds) ] ] =>
-        replace (open_defs z (subst_defs x y ds)) with (open_defs (subst_fvar x y z) (subst_defs x y ds))
-          by (unfold subst_fvar; rewrite~ If_r);
+        replace (open_defs z (subst_defs x y ds)) with (open_defs (subst_var x y z) (subst_defs x y ds))
+          by (unfold subst_var; rewrite~ If_r);
         rewrite_all <- subst_open_commut_defs
      | [ |- context [ open_trm ?z (subst_trm ?x ?y ?t) ] ] =>
-        replace (open_trm z (subst_trm x y t)) with (open_trm (subst_fvar x y z) (subst_trm x y t))
-          by (unfold subst_fvar; rewrite~ If_r);
+        replace (open_trm z (subst_trm x y t)) with (open_trm (subst_var x y z) (subst_trm x y t))
+          by (unfold subst_var; rewrite~ If_r);
         rewrite_all <- subst_open_commut_trm
     end.
 
@@ -377,7 +422,7 @@ Ltac subst_open_fresh :=
 Lemma subst_label_of_def: forall x y d,
   label_of_def d = label_of_def (subst_def x y d).
 Proof.
-  intros. destruct d; reflexivity.
+  intros. destruct* d.
 Qed.
 
 (** [l \notin labels(ds)]     #<br>#
@@ -387,10 +432,9 @@ Lemma subst_defs_hasnt: forall x y l ds,
   defs_hasnt ds l ->
   defs_hasnt (subst_defs x y ds) l.
 Proof.
-  intros x y l ds. unfold defs_hasnt. induction ds; introv Eq.
-  - reflexivity.
-  - unfold get_def. simpl. rewrite <- subst_label_of_def.
-    simpl in Eq. case_if~.
+  intros x y l ds. unfold defs_hasnt. induction ds; introv Eq; auto.
+  unfold get_def. simpl. rewrite <- subst_label_of_def.
+  simpl in Eq. case_if~.
 Qed.
 
 Ltac subst_fresh_solver :=
@@ -404,7 +448,7 @@ Ltac subst_fresh_solver :=
     rewrite <- concat_assoc; rewrite B;
     try match goal with
             | [ |- _; _; _; _ ⊢ _ _ _ :: _ ] =>
-              assert (z = subst_fvar x y z) as Hxyz by (unfold subst_fvar; rewrite~ If_r);
+              assert (z = subst_var x y z) as Hxyz by (unfold subst_var; rewrite~ If_r);
                 rewrite Hxyz at 1
             end;
     apply~ H;
@@ -460,42 +504,40 @@ Ltac subst_tydef_solver :=
     [G1, G2[y/x] ⊢ T[y/x] <: U[y/x]] #<br>#  #<br># *)
 
 (** The proof is by mutual induction on term typing, definition typing, and subtyping. *)
-Lemma subst_rules: forall y S,
+Lemma subst_rules: forall p S,
   (forall G t T, G ⊢ t : T -> forall G1 G2 x,
     G = G1 & x ~ S & G2 ->
     ok (G1 & x ~ S & G2) ->
     x \notin fv_ctx_types G1 ->
-    G1 & (subst_ctx x y G2) ⊢ tvar y : subst_typ x y S ->
-    G1 & (subst_ctx x y G2) ⊢ subst_trm x y t : subst_typ x y T) /\
+    G1 & (subst_ctx x p G2) ⊢ trm_path p : subst_typ x p S ->
+    G1 & (subst_ctx x p G2) ⊢ subst_trm x p t : subst_typ x p T) /\
   (forall z bs P G d D, z; bs; P; G ⊢ d : D -> forall G1 G2 x,
     G = G1 & x ~ S & G2 ->
     ok (G1 & x ~ S & G2) ->
     x \notin fv_ctx_types G1 ->
     x <> z ->
-    y <> z ->
-    G1 & (subst_ctx x y G2) ⊢ tvar y : subst_typ x y S ->
-    subst_var x y z; bs; P; G1 & (subst_ctx x y G2) ⊢ subst_def x y d : subst_dec x y D) /\
+    G1 & (subst_ctx x p G2) ⊢ trm_path p : subst_typ x p S ->
+    z; bs; P; G1 & (subst_ctx x p G2) ⊢ subst_def x p d : subst_dec x p D) /\
   (forall z bs P G ds T, z; bs; P; G ⊢ ds :: T -> forall G1 G2 x,
     G = G1 & x ~ S & G2 ->
     ok (G1 & x ~ S & G2) ->
     x \notin fv_ctx_types G1 ->
     x <> z ->
-    y <> z ->
-    G1 & (subst_ctx x y G2) ⊢ tvar y : subst_typ x y S ->
-    subst_var x y z; bs; P; G1 & (subst_ctx x y G2) ⊢ subst_defs x y ds :: subst_typ x y T) /\
+    G1 & (subst_ctx x p G2) ⊢ trm_path p : subst_typ x p S ->
+    z; bs; P; G1 & (subst_ctx x p G2) ⊢ subst_defs x p ds :: subst_typ x p T) /\
   (forall G T U, G ⊢ T <: U -> forall G1 G2 x,
     G = G1 & x ~ S & G2 ->
     ok (G1 & x ~ S & G2) ->
     x \notin fv_ctx_types G1 ->
-    G1 & (subst_ctx x y G2) ⊢ tvar y : subst_typ x y S ->
-    G1 & (subst_ctx x y G2) ⊢ subst_typ x y T <: subst_typ x y U).
+    G1 & (subst_ctx x p G2) ⊢ trm_path p : subst_typ x p S ->
+    G1 & (subst_ctx x p G2) ⊢ subst_typ x p T <: subst_typ x p U).
 Proof.
   introv. apply rules_mutind; intros; subst; simpl;
             try (subst_fresh_solver || rewrite subst_open_commut_typ_p);
             simpl in *; autounfold; eauto 4.
   - Case "ty_var".
     cases_if.
-    + apply binds_middle_eq_inv in b; subst; assumption.
+    + apply binds_middle_eq_inv in b; subst; auto. Admitted. (*
     + eapply subst_fresh_ctx in H1.
       apply binds_subst in b; auto.
       constructor. rewrite <- H1.
@@ -517,24 +559,21 @@ Proof.
     admit. (*constructor*.
     rewrite <- subst_label_of_def.
     apply subst_defs_hasnt. assumption.*)
-Qed.
+Qed.*)
 
 (** The substitution lemma for term typing.
     This lemma corresponds to Lemma 3.14 in the paper. *)
-Lemma subst_ty_trm: forall y S G x t T,
+Lemma subst_ty_trm: forall p S G x t T,
     G & x ~ S ⊢ t : T ->
     ok (G & x ~ S) ->
     x \notin fv_ctx_types G ->
-    G ⊢ tvar y : subst_typ x y S ->
-    G ⊢ subst_trm x y t : subst_typ x y T.
+    G ⊢ trm_path p : subst_typ x p S ->
+    G ⊢ subst_trm x p t : subst_typ x p T.
 Proof.
   intros.
-  apply (proj51 (subst_rules y S)) with (G1:=G) (G2:=empty) (x:=x) in H.
+  apply (proj51 (subst_rules p S)) with (G1:=G) (G2:=empty) (x:=x) in H.
   unfold subst_ctx in H. rewrite map_empty, concat_empty_r in H.
-  apply H.
-  rewrite concat_empty_r. reflexivity.
-  rewrite concat_empty_r. assumption.
-  assumption.
+  apply H. rewrite* concat_empty_r. rewrite* concat_empty_r. assumption.
   unfold subst_ctx. rewrite map_empty, concat_empty_r. assumption.
 Qed.
 
